Cpc/Proofs/Translation/Full.lean
@@ -763,7 +763,8 @@ theorem eo_to_smt_typeof_matches_translation
             (eo_to_smt_type_typeof_uconst i T).symm
     | Term.Apply f x, hNonNone => by
         haveI : TranslationBridge := ⟨go⟩
-        exact eo_to_smt_typeof_matches_translation_apply f x (go f) (go x) hNonNone
+        exact eo_to_smt_typeof_matches_translation_apply f x (go f) (go x)
+          (fun t _ hNN => go t hNN) hNonNone
     | Term._at_purify x, hNonNone => by
         exact eo_to_smt_typeof_matches_translation_purify x (go x hNonNone)
     | Term._at_array_deq_diff x1 x2, hNonNone => by
@@ -1037,7 +1038,7 @@ theorem eo_to_smt_typeof_matches_translation
         subst_vars
         simp_wf
       all_goals
-        sorry
+        omega
   exact go t
 
 /--
